test/generated.dfy
@@ -1,18 +1,39 @@
-
-
 datatype tree<a1> =  Node(a1, tree<a1>, tree<a1>) |  Nil
-function repr(xre : tree<int>) : tree<int>  {xre}
-function spec(xsp : tree<int>) : int  {f(0, xsp)}
+
+function repr(xre : tree<int>) : tree<int>  
+{
+  xre
+}
+function spec(xsp : tree<int>) : int  
+{
+  f(0, xsp)
+}
 function f(x5 : int, x6 : tree<int>) : int 
-  {match x6
-case Nil =>  x5
-case Node(a, l, r) =>  ((sum) => f(sum + a, r))(
-                                                  f(x5, l))}
+// decreases x6
+{
+  match x6
+  case Nil =>  x5
+  case Node(a, l, r) => 
+    ((sum) => f(sum + a, r))(f(x5, l))
+  
+}
 function target(xtarg : tree<int>) : int 
-  {match xtarg
-case Nil =>  s0
-case Node(a, l, r) =>  join(a, target(l),
-                                                     target(r))}
-function s0() : int  {0}
-function join(x2 : int, x3 : int, x4 : int) : int  {x3 + x2 + x4}
-lemma correctness_lemma(x : tree)  ensures (target(x) == spec(repr(x))) {}
+// decreases xtarg
+{
+  match xtarg
+  case Nil => 0
+  case Node(a, l, r) =>  join(a, target(l), target(r))
+}
+function join(x2 : int, x3 : int, x4 : int) : int
+{
+  x3 + x2 + x4
+}
+
+
+lemma correctness_lemma(x : tree<int>)
+ensures target(x) == spec(repr(x))
+{
+  match x
+  case Nil => {}
+  case Node(a, l, r) => {}
+}
